src/threadpool.v
@@ -11,72 +11,84 @@ From Paco Require Import paco.
 From Paco Require Import paco3.
 Import EqNotations.
 
-(** An event type transformer for adding concurrency. *)
-CoInductive threadpoolE (E : Type → Type) : Type → Type :=
-  | EEmit (A : Type) (e : E A) : threadpoolE E A
+(** Thread continuation. *)
+Variant thread :=
+ | CurrentThread
+ | NewThread.
+(** An event type for concurrency. *)
+Variant threadpoolE : Type → Type :=
+  (** Unix-style fork that splits the thread (copying its stack) into two
+  threads, distinguished by the answer value of type [[thread]]. Execution
+  continues in the thread with answer [CurrentThread] until a [EYield] is
+  emitted. *)
+  | EFork : threadpoolE thread
   (** Yield control to another (demonically chosen) thread in the thread-pool. *)
-  | EYield : threadpoolE E unit
-  (** Split the thread into two threads corresponding to the answers [true]
-  and [false]. *)
-  | EFork (t : itree (threadpoolE E) unit) : threadpoolE E unit.
-Arguments EEmit {_ _} _.
-Arguments EYield {_}.
-Arguments EFork {_} _.
+  | EYield : threadpoolE unit
+  (** (Safely) kill the current thread and yield. *)
+  | EKillThread : threadpoolE Empty_set.
+Arguments EYield.
+Arguments EFork.
+Arguments EKillThread.
 
-Global Instance E_threadpoolE (E : Type → Type) : Subevent E (threadpoolE E) :=
-  { resum := λ A e, EEmit e }.
-
-(** [iHandler] transformer for [threadpoolE]. *)
-Program Definition threadpoolH {Σ E} `{!invGS_gen HasNoLc Σ} (H : iHandler Σ E) : iHandler Σ (threadpoolE E) :=
+(** [iHandler] for [threadpoolE]. *)
+Program Definition threadpoolH {Σ} `{!invGS_gen HasNoLc Σ} : iHandler Σ threadpoolE :=
   IHandler (λ A e,
     match e with
-    | EEmit e' => λ Φ s, H _ e' Φ (λ t, s (translate (@EEmit _) t))
-    | EYield       => λ Φ s, |={∅, ⊤}=> |={⊤, ∅}=> Φ tt
-    | EFork t      => λ Φ s, Φ tt ∗ s t
+    (** We define the iHandler in a way that imposes a semantic restriction on
+    [EFork] disallowing returning in the [NewThread] continuation, even
+    though it is possible to define [itree]s that do so. From the point of view
+    of [WPi], we are thus declaring such returns as unsafe. This
+    overapproximation is justified from our applications. *)
+    | EFork      => λ Φ s, Φ CurrentThread ∗ s NewThread
+    | EYield     => λ Φ _, |={∅, ⊤}=> |={⊤, ∅}=> Φ tt
+    | EKillThread => λ _ _, |={∅, ⊤}=> True
     end
   )%I _.
 Next Obligation.
-  iIntros (??????????) "HΦwand #Hswand". destruct e.
-  - iIntros "HH". iApply (mono with "[HΦwand] [Hswand]"); last done.
-    * exact.
-    * iModIntro. iIntros (t) "Hs". by iApply "Hswand".
-  - iIntros "HΦfupd". by iApply "HΦwand".
-  - iIntros "[HΦ Hs]". iSplitL "HΦ HΦwand".
+  iIntros (????????) "HΦwand #Hswand". destruct e.
+  - iIntros "[HΦ Hs]". iSplitL "HΦwand HΦ".
     * by iApply "HΦwand".
     * by iApply "Hswand".
-Qed.
-
-Global Instance threadpoolE_inH `{!invGS_gen HasNoLc Σ} (E : Type → Type) (H : iHandler Σ E) :
-  inH H (threadpoolH H).
-Proof.
-  by intros.
+  - iIntros "HΦ". by iApply "HΦwand".
+  - by iIntros "?".
 Qed.
 
 Section wp_threadpool.
   Context `{!invGS_gen HasNoLc Σ} {E : Type → Type} {H : iHandler Σ E}.
+  Context `{threadpoolE -< E} `{inH Σ threadpoolE E threadpoolH H}.
 
-  Lemma wpi_fork {R} (t : itree (threadpoolE E) unit) (k : unit → itree (threadpoolE E) R) (M : coPset) (Φ : R → iProp Σ) :
-    (▷ WPi (k tt) @ threadpoolH H; M {{ Φ }} ∗ ▷ WPi t @ threadpoolH H; ⊤ {{ _, True }}) -∗
-    WPi (Vis (EFork t) k) @ threadpoolH H; M {{ Φ }}.
+  Lemma wpi_fork {R} (k : thread → itree E R) (M : coPset) (Φ : R → iProp Σ) :
+    (▷ WPi (k CurrentThread) @ H; M {{ Φ }} ∗ ▷ WPi (k NewThread) @ H; ⊤ {{ _, False }}) -∗
+    WPi (vis EFork k) @ H; M {{ Φ }}.
   Proof.
-    iIntros "[Hwp1 Hwp2]". iApply wpi_vis.
+    iIntros "[Hwpcur Hwpnew]". iApply wpi_vis.
     rewrite /threadpoolH. iFrame.
     iApply fupd_mask_intro; first apply empty_subseteq. iIntros "Hfupd".
-    iNext. rewrite -wpi_clear_mask. iMod "Hfupd". by iMod "Hwp1".
+    iApply is_inH. simpl. iSplitL "Hwpcur Hfupd".
+    - iNext. iMod "Hfupd". by iApply wpi_update_post_emp_mask.
+    - done.
   Qed.
 
   (** Note here crucially that the mask has to be full for the rule to apply.
   This means that you cannot step over an [EYield] if there are open
   invariants. It amounts to the typical requirement of atomicity in the
   invariant opening rule known from "normal Iris". *)
-  Lemma wpi_yield {R} (k : unit → itree (threadpoolE E) R) (M : coPset) (Φ : R → iProp Σ) :
-    (▷ WPi (k tt) @ threadpoolH H; ⊤ {{ Φ }}) -∗
-    WPi (Vis EYield k) @ threadpoolH H; ⊤ {{ Φ }}.
+  Lemma wpi_yield {R} (k : unit → itree E R) (M : coPset) (Φ : R → iProp Σ) :
+    (▷ WPi (k tt) @ H; ⊤ {{ Φ }}) -∗
+    WPi (vis EYield k) @ H; ⊤ {{ Φ }}.
   Proof.
-    iIntros "Hwp". iApply wpi_vis.
-    rewrite /threadpoolH. simpl. iApply fupd_mask_intro_subseteq; first done.
+    iIntros "Hwp". iApply wpi_vis. iApply is_inH. simpl.
+    iApply fupd_mask_intro_subseteq; first done.
     iApply fupd_mask_intro; first apply empty_subseteq. iIntros "Hfupd".
     iNext. rewrite -wpi_clear_mask. iMod "Hfupd". by iMod "Hwp".
+  Qed.
+
+  Lemma wpi_kill {R} (k : Empty_set → itree E R) (M : coPset) (Φ : R → iProp Σ) :
+    (|={∅, ⊤}=> True) -∗
+    WPi (vis EKillThread k) @ H; ⊤ {{ Φ }}.
+  Proof.
+    iIntros "Hwp". iApply wpi_vis. iApply is_inH. simpl.
+    by iApply fupd_mask_intro_subseteq; first done.
   Qed.
 End wp_threadpool.
 
@@ -117,9 +129,9 @@ Section interleaving.
   Context `{!invGS_gen HasNoLc Σ} {E : Type → Type} {H : iHandler Σ E}.
 
   Variant interleavesF
-    (interleaves : list (itree (threadpoolE E) unit) -> itree (threadpoolE E) unit -> itree E unit -> Prop)
-    :  list (itree (threadpoolE E) unit)
-    -> itree' (threadpoolE E) unit
+    (interleaves : list (itree (threadpoolE +' E) unit) -> itree (threadpoolE +' E) unit -> itree E unit -> Prop)
+    :  list (itree (threadpoolE +' E) unit)
+    -> itree' (threadpoolE +' E) unit
     -> itree' E unit
     -> Prop :=
   | Terminates :
@@ -128,24 +140,25 @@ Section interleaving.
     tp !! new_current_tid = Some new_current →
     interleaves (delete new_current_tid tp) new_current interleaving' →
     interleavesF interleaves tp (RetF tt) (TauF interleaving')
+  | KillThread tp k new_current_tid new_current interleaving' :
+    tp !! new_current_tid = Some new_current →
+    interleaves (delete new_current_tid tp) new_current interleaving' →
+    interleavesF interleaves tp (VisF (inl1 EKillThread) k) (TauF interleaving')
   | Steps current' tp interleaving' :
     interleaves tp current' interleaving' →
     interleavesF interleaves tp (TauF current') (TauF interleaving')
-  | Emits tp A e k k' :
-    (∀ a, interleaves tp (k' a) (k a)) →
-    interleavesF interleaves tp (VisF (@EEmit E A e) k') (VisF e k)
   | Yields tp k new_current_tid new_current interleaving' :
     tp !! new_current_tid = Some new_current →
     interleaves (cons (Tau (k tt)) (delete new_current_tid tp)) new_current interleaving' →
-    interleavesF interleaves tp (VisF EYield k) (TauF interleaving')
-  | Forks tp t k interleaving' :
-    interleaves (cons t tp) (k tt) interleaving' →
-    interleavesF interleaves tp (VisF (EFork t) k) (TauF interleaving').
+    interleavesF interleaves tp (VisF (inl1 EYield) k) (TauF interleaving')
+  | Forks tp k interleaving' :
+    interleaves (cons (k NewThread) tp) (k CurrentThread) interleaving' →
+    interleavesF interleaves tp (VisF (inl1 EFork) k) (TauF interleaving').
   Hint Constructors interleavesF : iris_itree.
   Definition interleaves_
-    (interleaves : list (itree (threadpoolE E) unit) -> itree (threadpoolE E) unit -> itree E unit -> Prop)
-    :  list (itree (threadpoolE E) unit)
-    -> itree (threadpoolE E) unit
+    (interleaves : list (itree (threadpoolE +' E) unit) -> itree (threadpoolE +' E) unit -> itree E unit -> Prop)
+    :  list (itree (threadpoolE +' E) unit)
+    -> itree (threadpoolE +' E) unit
     -> itree E unit
     -> Prop :=
     fun tp current interleaving =>
@@ -166,54 +179,61 @@ Section interleaving.
   Hint Resolve interleaves__mono : paco.
 
   Definition interleaves :
-    list (itree (threadpoolE E) unit) -> itree (threadpoolE E) unit -> itree E unit -> Prop :=
+    list (itree (threadpoolE +' E) unit) -> itree (threadpoolE +' E) unit -> itree E unit -> Prop :=
     paco3 interleaves_ bot3.
 
   Theorem wpi_interleaving'
-    (tp : list (itree (threadpoolE E) unit))
-    (current : itree (threadpoolE E) unit)
+    (tp : list (itree (threadpoolE +' E) unit))
+    (current : itree (threadpoolE +' E) unit)
     (interleaving : itree E unit) :
     interleaves tp current interleaving →
-    ([∗ list] thread ∈ tp, WPi thread @ threadpoolH H; ⊤ {{ _, True }}) -∗
-    WPi current @ threadpoolH H; ∅ {{ _, |={∅, ⊤}=> True }} -∗
+    ([∗ list] thread ∈ tp, WPi thread @ threadpoolH ⊕ H; ⊤ {{ _, True }}) -∗
+    WPi current @ threadpoolH ⊕ H; ∅ {{ _, |={∅, ⊤}=> True }} -∗
     WPi interleaving @ H; ∅ {{ _, |={∅, ⊤}=> True }}.
   Proof.
     iIntros "%Hinter Htp Hcurrent".
     iLöb as "IH" forall (tp current interleaving Hinter). punfold Hinter.
-    inversion Hinter as [Heqtp Heqcurrent Heqinterleaving|tp' new_current_tid new_current interleaving' Hidx Hinter' Heqtp Heqcurrent Heqinterleaving|current' tp' interleaving' Hinter' Heqtp Heqcurrent Heqinterleaving|tp' A e k k' Hinter' Heqtp Heqcurrent Heqinterleaving|tp' k new_current_tid new_current interleaving' Hidx Hinter' Heqtp Heqcurrent Heqinterleaving|tp' t k interleaving' Hinter' Heqtp Heqcurrent Heqinterleaving].
+    inversion Hinter as
+      [Heqtp Heqcurrent Heqinterleaving
+      |tp' new_current_tid new_current interleaving' Hidx Hinter' Heqtp Heqcurrent Heqinterleaving
+      |tp' k new_current_tid new_current interleaving' Hidx Hinter' Heqtp Heqcurrent Heqinterleaving
+      |current' tp' interleaving' Hinter' Heqtp Heqcurrent Heqinterleaving
+      |tp' k new_current_tid new_current interleaving' Hidx Hinter' Heqtp Heqcurrent Heqinterleaving
+      |tp' k interleaving' Hinter' Heqtp Heqcurrent Heqinterleaving
+      ].
     - apply ret_observe_eqit in Heqcurrent as <-. apply ret_observe_eqit in Heqinterleaving as <-.
       by rewrite -!wpi_ret'.
     - apply ret_observe_eqit in Heqcurrent as <-. apply tau_observe_eqit in Heqinterleaving as <-.
       iApply wpi_tau. iNext.
       iDestruct (big_sepL_delete' _ _ _ new_current_tid with "Htp") as "[Hcurrent' Htp']"; first done.
-      unfold bot3, upaco3 in Hinter'. destruct Hinter' as [Hinter'|]; last contradiction.
-      iApply ("IH" with "[] [Htp']").
+      destruct Hinter' as [Hinter'|]; last contradiction. iApply ("IH" with "[] [Htp']").
       * done.
       * done.
       * rewrite -wpi_ret'. iMod "Hcurrent". iMod "Hcurrent".
+        iDestruct (wpi_clear_mask with "Hcurrent'") as "Hcurrent'". by do 2 iMod "Hcurrent'".
+    - apply vis_observe_eqit in Heqcurrent as <-. apply tau_observe_eqit in Heqinterleaving as <-.
+      rewrite -wpi_vis'. simpl. iApply wpi_tau. iNext.
+      iDestruct (big_sepL_delete' _ _ _ new_current_tid with "Htp") as "[Hcurrent' Htp']"; first done.
+      destruct Hinter' as [Hinter'|]; last contradiction.
+      iApply ("IH" with "[] [Htp']").
+      * done.
+      * done.
+      * iMod "Hcurrent". simpl. iMod "Hcurrent".
         iDestruct (wpi_clear_mask with "Hcurrent'") as "Hcurrent'". by do 2 iMod "Hcurrent'".
     - apply tau_observe_eqit in Heqcurrent as <-. apply tau_observe_eqit in Heqinterleaving as <-.
       rewrite -!wpi_tau'. iMod (fupd_mask_subseteq ∅) as "Hfupd"; first done. iMod "Hcurrent".
       iModIntro. iNext. iMod "Hfupd".
       iEval (rewrite wpi_update_post). iApply ("IH" with "[] [Htp]").
-      * unfold bot3, upaco3 in Hinter'. by destruct Hinter'.
+      * by destruct Hinter'.
       * done.
       * rewrite !wpi_update_post //.
-    - apply vis_observe_eqit in Heqcurrent as <-. apply vis_observe_eqit in Heqinterleaving as <-.
-      rewrite -!wpi_vis'. iMod (fupd_mask_subseteq ∅) as "Hfupd"; first done. iMod "Hcurrent".
-      iApply (mono with "[Hfupd Htp] [] [Hcurrent]"); last done.
-      * iIntros (a) "Hwp". iNext. iMod "Hfupd".
-        iEval (rewrite wpi_update_post). iApply ("IH" with "[] Htp").
-        + unfold bot3, upaco3 in Hinter'. by destruct (Hinter' a).
-        + rewrite wpi_update_post //.
-      * iModIntro. iIntros (t) "Hwp". iNext. by iApply wpi_inH.
     - apply vis_observe_eqit in Heqcurrent as <-. apply tau_observe_eqit in Heqinterleaving as <-.
       iApply wpi_tau'. rewrite -wpi_vis'. simpl. do 2 iMod "Hcurrent".
       rewrite wpi_update_post wpi_tau'.
       iDestruct (big_sepL_delete' _ _ _ new_current_tid with "Htp") as "[Hcurrent' Htp']"; first done.
       iMod (fupd_mask_subseteq ∅) as "Hfupd"; first done. iModIntro. iNext.
       iApply wpi_update_post. iApply ("IH" with "[] [Hcurrent Htp']").
-      * unfold bot3, upaco3 in Hinter'. by destruct Hinter'.
+      * by destruct Hinter'.
       * iApply big_sepL_cons.
         iSplitL "Hcurrent".
         + iMod (fupd_mask_subseteq ∅) as "Hfupd"; first done. by iMod "Hfupd".
@@ -223,15 +243,15 @@ Section interleaving.
     - apply vis_observe_eqit in Heqcurrent as <-. apply tau_observe_eqit in Heqinterleaving as <-.
       iApply wpi_tau'. rewrite -wpi_vis'. simpl. iMod "Hcurrent" as "[Hforked Hcurrent']".
       iModIntro. iNext. iApply wpi_update_post. iApply ("IH" with "[] [Hcurrent' Htp]").
-      * unfold bot3, upaco3 in Hinter'. by destruct Hinter'.
-      * iApply big_sepL_cons. iFrame.
+      * by destruct Hinter'.
+      * iApply big_sepL_cons. iFrame. iApply wpi_wand; last done. by iIntros (?) "?".
       * rewrite wpi_update_post //.
   Qed.
   Corollary wpi_interleaving
-    (concurrent : itree (threadpoolE E) unit)
+    (concurrent : itree (threadpoolE +' E) unit)
     (interleaving : itree E unit) :
     interleaves [] concurrent interleaving →
-    WPi concurrent @ threadpoolH H; ⊤ {{ _, True }} -∗
+    WPi concurrent @ threadpoolH ⊕ H; ⊤ {{ _, True }} -∗
     WPi interleaving @ H; ⊤ {{ _, True }}.
   Proof.
     iIntros "%Hinter Hwp". iApply wpi_clear_mask.
